-

Determinant.v
@@ -1597,7 +1597,7 @@ Qed.
 
 Definition is_permut {n} (σ : vector n nat) :=
   (∀ i, i < n → vect_el σ i < n) ∧
-  (∀ i j, i < n → j < n → i ≠ j → vect_el σ i ≠ vect_el σ j).
+  (∀ i j, i < n → j < n → vect_el σ i = vect_el σ j → i = j).
 
 Fixpoint permut_find n (σ : vector n nat) i j :=
   match i with
@@ -1605,13 +1605,16 @@ Fixpoint permut_find n (σ : vector n nat) i j :=
   | S i' => if Nat.eq_dec (vect_el σ i') j then i' else permut_find σ i' j
   end.
 
+Definition permut_inv' n (σ : vector n nat) := mk_vect n (permut_find σ n).
+
+(*
 Fixpoint permut_fun_find (f : nat → nat) n i :=
   match n with
   | 0 => 42
   | S n' => if Nat.eq_dec (f n') i then n' else permut_fun_find f n' i
   end.
 
-Theorem permut_permut_fun_find : ∀ n (σ : vector n nat) i j,
+Theorem permut_list_find : ∀ n (σ : vector n nat) i j,
   permut_find σ i j = permut_fun_find (vect_el σ) i j.
 Proof.
 intros.
@@ -1620,12 +1623,55 @@ destruct (Nat.eq_dec (vect_el σ i) j) as [Hij| Hij]; [ easy | ].
 apply IHi.
 Qed.
 
-Definition permut_inv n (σ : vector n nat) := mk_vect n (permut_find σ n).
-
-(*
-Compute let n := 5 in let k := 3 in (list_of_vect (canon_permut n k), list_of_vect (permut_inv (canon_permut n k))).
-Compute let n := 4 in map (λ k, list_of_vect (permut_inv (canon_permut n k))) (seq 0 (fact n)).
+Theorem permut_list_find : ∀ n (σ : vector n nat) i,
+  is_permut σ
+  → permut_find σ n i =
+    match find (λ j, j =? i) (list_of_vect σ) with
+    | None => 42
+    | Some j => j
+    end.
+Proof.
+intros * (Hp1, Hp2).
+unfold list_of_vect.
+remember (vect_el σ) as f eqn:Hf.
+Print permut_find.
+...
+revert i.
+induction n; intros; [ easy | cbn ].
+destruct (Nat.eq_dec (vect_el σ n) i) as [Hni| Hni]. {
+  cbn.
+  remember (vect_el σ 0 =? i) as b eqn:Hb; symmetry in Hb.
+  destruct b. {
+    apply Nat.eqb_eq in Hb.
+    rewrite <- Hni in Hb.
+    apply Hp2 in Hb; [ subst n | flia | flia ].
+    specialize (Hp1 0 Nat.lt_0_1).
+    now apply Nat.lt_1_r in Hp1.
+  } {
+    apply Nat.eqb_neq in Hb.
+Search (find _ (map _ _)).
+...
+induction i; [ easy | cbn ].
+destruct (Nat.eq_dec (vect_el σ i) j) as [Hij| Hij]; [ easy | ].
+apply IHi.
+Qed.
 *)
+
+Definition permut_inv n (σ : vector n nat) :=
+  mk_vect n
+    (λ i,
+     match find (Nat.eqb i) (list_of_vect σ) with
+     | None => 42
+     | Some j => j
+     end).
+
+(**)
+Compute let n := 5 in let k := 3 in (list_of_vect (canon_permut n k), list_of_vect (permut_inv (canon_permut n k))).
+Compute let n := 5 in let k := 3 in (list_of_vect (canon_permut n k), list_of_vect (permut_inv' (canon_permut n k))).
+Compute let n := 4 in map (λ k, list_of_vect (permut_inv (canon_permut n k))) (seq 0 (fact n)).
+Compute let n := 4 in map (λ k, list_of_vect (permut_inv' (canon_permut n k))) (seq 0 (fact n)).
+...
+(**)
 
 (*
 Theorem glop : ∀ f i k n,
@@ -1670,6 +1716,7 @@ Theorem permut_inv_prop : ∀ n (σ : vector n nat) i,
   → vect_el σ (vect_el (permut_inv σ) i) = i.
 Proof.
 intros * (Hp1, Hp2) Hin; cbn.
+...
 rewrite permut_permut_fun_find.
 remember (vect_el σ) as f eqn:Hf.
 clear σ Hf.
